restore Invariant.fst

pulse/lib/pulse/lib/Pulse.Lib.Reference.fst
@@ -27,6 +27,7 @@ let pts_to
     (#[exact (`full_perm)] [@@@equate_by_smt] p:perm)
     ([@@@equate_by_smt] v:a)
   = H.pts_to r #p (U.raise_val v)
+let pts_to_is_small r p x = H.pts_to_is_small r p (U.raise_val x)
 
 ```pulse
 fn alloc' (#a:Type u#0) (v:a)
