pulse/lib/pulse/lib/Pulse.Lib.HigherReference.fsti
@@ -24,6 +24,9 @@ val ref ([@@@unused]a:Type u#1) : Type u#0
 
 val pts_to (#a:Type) (r:ref a) (#[T.exact (`full_perm)] p:perm) (n:a) : vprop
 
+val pts_to_is_small (#a:Type) (r:ref a) (p:perm) (n:a)
+  : Lemma (is_small (pts_to r #p n))
+
 val alloc (#a:Type) (x:a)
   : stt (ref a) emp (fun r -> pts_to r x)
 
